'Builder' 를 잘못 정의한 것 같은데! - 'SortList' 는 밖에 있어야지!

Nemonuri/Functions/LiftableEmbedding/Interleaving.lean
@@ -9,6 +9,235 @@ set_option autoImplicit false
 namespace Nemonuri.Functions.LiftableEmbedding
 
 
+inductive Interleaving.{uu, us} (Univ: Sort uu) : List (Sort us) → Sort _ where
+  | nil: Interleaving Univ []
+  | cons {sub: Sort us} (lem: LiftableEmbedding sub Univ) {subs: List (Sort us)} : Interleaving Univ subs → Interleaving Univ (sub::subs)
+
+namespace Interleaving
+
+universe uu us
+variable {Univ: Sort uu} {ss: List (Sort us)}
+
+def subs (_: Interleaving Univ ss) : List (Sort us) := ss
+
+def length (il: Interleaving Univ ss) : Nat := il.subs.length
+
+@[defeq]
+theorem length_def {il: Interleaving Univ ss} : il.length = ss.length := rfl
+
+@[defeq]
+theorem nil_length_eq_zero : (.nil : Interleaving Univ []).length = 0 := by
+  dsimp [length_def]
+
+instance nil_subsingleton : Subsingleton (Interleaving Univ []) where
+  allEq := by rintro ⟨⟩ ⟨⟩; rfl
+
+@[defeq]
+theorem cons_length_eq {s: Sort us} {lem: LiftableEmbedding s Univ} {ss: List (Sort us)} {il: Interleaving Univ ss}
+  : (cons lem il).length = il.length + 1 := by
+  dsimp [length_def]
+
+
+def GetSub (il: Interleaving Univ ss) (n: Fin il.length) : Sort us := il.subs.get n
+
+@[defeq]
+theorem cons_getSub_eq {s: Sort us} {lem: LiftableEmbedding s Univ} {ss: List (Sort us)} {il: Interleaving Univ ss} {n: Fin il.length}
+  : (cons lem il).GetSub (Fin.mk (n+1) (by simp [cons_length_eq])) = il.GetSub n := by
+  dsimp [GetSub, subs]
+
+
+def getLiftableEmbeddingAt (ss: List (Sort us)) (il: Interleaving Univ ss) (n: Fin il.length) : LiftableEmbedding (il.GetSub n) Univ :=
+  match ss, il with
+  | [], .nil => Fin.elim0 (nil_length_eq_zero ▸ n)
+  | s::ss, .cons lem il =>
+  match n with
+  | ⟨0, _⟩ => lem
+  | ⟨n+1, lm1⟩ =>
+    have lm2: n < il.length := by simpa [cons_length_eq] using lm1
+    getLiftableEmbeddingAt ss il ⟨n, lm2⟩
+
+
+def getLiftableEmbedding (il: Interleaving Univ ss) (n: Fin il.length) : LiftableEmbedding (il.GetSub n) Univ := il.getLiftableEmbeddingAt ss n
+
+
+inductive MapsToIsLiftable {Univ: Sort uu} (uv: Univ) : {ss: List (Sort us)} → Interleaving Univ ss → List Bool → Prop where
+  | nil : MapsToIsLiftable uv (.nil) []
+  | cons_true {s: Sort us} (lem: LiftableEmbedding s Univ) {ss: List (Sort us)} (il: Interleaving Univ ss) (req: lem.IsLiftable uv) (bs: List Bool)
+        : il.MapsToIsLiftable uv bs → (il.cons lem).MapsToIsLiftable uv (.true::bs)
+  | cons_false {s: Sort us} (lem: LiftableEmbedding s Univ) {ss: List (Sort us)} (il: Interleaving Univ ss) (req: ¬lem.IsLiftable uv) (bs: List Bool)
+        : il.MapsToIsLiftable uv bs → (il.cons lem).MapsToIsLiftable uv (.false::bs)
+
+
+namespace MapsToIsLiftable
+
+theorem length_eq_at (uv: Univ) (ss: List (Sort us)) (bs: List Bool) (il: Interleaving Univ ss) (h: il.MapsToIsLiftable uv bs) : il.length = bs.length := by
+  dsimp [il.length_def]
+  cases ss with
+  | nil =>
+    cases bs with
+    | nil => dsimp
+    | cons b bs => rcases h
+  | cons s ss =>
+    cases bs with
+    | nil => rcases h
+    | cons b bs =>
+      simp
+      cases h <;> (
+        rename_i il h
+        rewrite [← il.length_def]
+        exact h.length_eq_at )
+
+variable {il: Interleaving Univ ss} {uv: Univ} in
+theorem length_eq {bs: List Bool} (h: il.MapsToIsLiftable uv bs) : il.length = bs.length := h.length_eq_at
+
+
+theorem bool_list_eq_at (uv: Univ) (ss: List (Sort us)) (il: Interleaving Univ ss) (bs1: List Bool) (h1: il.MapsToIsLiftable uv bs1) (bs2: List Bool) (h2: il.MapsToIsLiftable uv bs2) : bs1 = bs2 := by
+  have lm1 := h1.length_eq.symm.trans h2.length_eq
+  rcases bs1 with _ | ⟨b1, bs1⟩
+  · simp at lm1
+    replace lm1 := lm1.symm
+    simpa using lm1
+  · simp at lm1
+    rcases bs2 with _ | ⟨b2, bs2⟩
+    · simp at lm1
+    · simp at lm1 ⊢
+      rcases b1 <;> rcases b2
+      · simp only [true_and]
+        rcases h1; rename_i il _ h1
+        rcases h2; rename_i h2
+        exact bool_list_eq_at uv _ il _ h1 _ h2
+      · rcases h1; rcases h2
+        contradiction
+      · rcases h1; rcases h2
+        contradiction
+      · simp only [true_and]
+        rcases h1; rename_i il _ h1
+        rcases h2; rename_i h2
+        exact bool_list_eq_at uv _ il _ h1 _ h2
+
+
+variable {il: Interleaving Univ ss} {uv: Univ} in
+theorem bool_list_eq {bs1 bs2: List Bool} (h1: il.MapsToIsLiftable uv bs1) (h2: il.MapsToIsLiftable uv bs2) : bs1 = bs2 := bool_list_eq_at _ _ _ _ h1 _ h2
+
+
+
+end MapsToIsLiftable
+
+def AnyLiftable (il: Interleaving Univ ss) (uv: Univ) : Prop := ∀⦃bs: List Bool⦄ ⦃_: il.MapsToIsLiftable uv bs⦄, bs.Mem .true
+
+def AllLiftable (il: Interleaving Univ ss) (uv: Univ) : Prop := ∀⦃bs: List Bool⦄ ⦃_: il.MapsToIsLiftable uv bs⦄, bs.Forall (· = .true)
+
+
+structure Builder (Univ: Sort uu) (len: Nat) where
+  GetSub (n: Fin len) : Sort us
+  getLiftableEmbedding (n: Fin len) : LiftableEmbedding (GetSub n) Univ
+
+namespace Builder
+
+
+def nil (Univ: Sort uu) : Builder.{uu, us} Univ 0 where
+  GetSub n := n.elim0
+  getLiftableEmbedding n := n.elim0
+
+instance zero_subsingleton : Subsingleton (Builder Univ 0) where
+  allEq := by
+    rintro ⟨gs1, gl1⟩ ⟨gs2, gl2⟩
+    have lm1: gs1 = gs2 := by simp [funext_iff]
+    subst lm1
+    simp [funext_iff]
+
+
+def cons (Sub: Sort us) (lem: LiftableEmbedding Sub Univ) {len: Nat} (bd: Builder Univ len) : Builder Univ (len+1) :=
+  let getSub (n: Fin (len + 1)) : Sort us := n.induction Sub (fun n0 _ => bd.GetSub n0)
+  have lm1 : getSub 0 = Sub := Fin.induction_zero _ _
+  {
+    GetSub := getSub
+    getLiftableEmbedding (n: Fin (len + 1)) :=
+      n.induction (motive := fun n0 => LiftableEmbedding (getSub n0) Univ)
+                  (lm1.symm ▸ lem)
+                  (fun n0 _ =>
+                    have lm2: bd.GetSub n0 = getSub (n0.succ) := by subst getSub; simp only [Fin.induction_succ]
+                    lm2 ▸ (bd.getLiftableEmbedding n0))
+  }
+
+
+def tail {len: Nat} (bd: Builder Univ (len+1)) : Builder Univ len where
+  GetSub n := bd.GetSub n.succ
+  getLiftableEmbedding n := bd.getLiftableEmbedding n.succ
+
+@[elab_as_elim]
+def recCons.{u} {len: Nat}
+  {motive: Builder Univ (len+1) → Sort u}
+  (cons: (Sub: Sort us) → (lem: LiftableEmbedding Sub Univ) → (bd: Builder Univ len) → motive (.cons Sub lem bd))
+  (t: Builder Univ (len+1))
+  : motive t :=
+    let Sub : Sort us := t.GetSub 0
+    let lem : LiftableEmbedding Sub Univ := t.getLiftableEmbedding 0
+    have lm1: Builder.cons Sub lem t.tail = t := by
+      subst Sub lem
+      rcases t with ⟨gs, gl⟩
+      dsimp [Builder.cons, Builder.tail]
+      simp
+      refine (And.intro ?_ ?_)
+      · simp [funext_iff]
+        intro n0
+        cases n0 using Fin.succRec <;> dsimp
+      · refine Function.hfunext (Eq.refl _) ?_
+        intro n1 n2 lm1
+        rewrite [heq_eq_eq] at lm1
+        subst lm1
+        cases n1 using Fin.succRec <;> (dsimp; rfl)
+    lm1.ndrec (cons Sub lem t.tail)
+
+@[elab_as_elim]
+def recNilCons.{u}
+  {motive : (len: Nat) → Builder Univ len → Sort u}
+  (nil: motive 0 (.nil Univ))
+  (cons: (Sub: Sort us) → (lem: LiftableEmbedding Sub Univ) → (len: Nat) → (bd: Builder Univ len) → motive (len+1) (.cons Sub lem bd))
+  {len: Nat} (t: Builder Univ len)
+  : motive len t :=
+  match len with
+  | 0 =>
+    have lm1: Builder.nil Univ = t := zero_subsingleton.elim _ _
+    lm1.ndrec nil
+  | len + 1 =>
+    t.recCons (fun Sub lem bd => cons Sub lem len bd)
+
+
+def toInterleavingAt (len: Nat) (bd: Builder Univ len) : Interleaving Univ (List.ofFn bd.GetSub) :=
+  match len, bd with
+  | 0, _ => (.nil: Interleaving Univ [])
+  | len+1, bd2 => bd2.recCons (fun Sub lem bd0 =>
+      have lm1: Sub :: List.ofFn bd0.GetSub = List.ofFn (bd0.cons Sub lem).GetSub := by simp [cons]
+      lm1.ndrec (Interleaving.cons lem (toInterleavingAt len bd0)))
+
+def toInterleaving {len: Nat} (bd: Builder Univ len) : Interleaving Univ (List.ofFn bd.GetSub) := bd.toInterleavingAt len
+
+
+def ofInterleaving (il: Interleaving Univ ss) : Builder Univ il.length where
+  GetSub := il.GetSub
+  getLiftableEmbedding := il.getLiftableEmbedding
+
+
+
+
+
+end Builder
+
+end Interleaving
+
+/-
+inductive IsLiftableVector (rv: R) : (bs: List (LeftTypeBundled.{ur, ul} R)) → (Interleaving R bs) → List Bool → Prop where
+  | nil : IsLiftableVector rv [] (Interleaving.nil) []
+  | cons_true (b: LeftTypeBundled R) (bs: List (LeftTypeBundled R)) (il: Interleaving R bs)
+              (b2: b.liftableEmbedding.IsLiftable rv) (bs2: List Bool)
+        : IsLiftableVector rv bs il bs2 → IsLiftableVector rv (b::bs) (il.cons b) (.true::bs2)
+  | cons_false (b: LeftTypeBundled R) (bs: List (LeftTypeBundled R)) (il: Interleaving R bs)
+               (b2: ¬b.liftableEmbedding.IsLiftable rv) (bs2: List Bool)
+        : IsLiftableVector rv bs il bs2 → IsLiftableVector rv (b::bs) (il.cons b) (.false::bs2)
+
+
+
 structure LeftTypeBundled.{ur, ul} (R: Type ur) where
   L: Type ul
   liftableEmbedding: LiftableEmbedding L R
@@ -30,18 +259,9 @@ universe ur ul
 
 variable {R: Type ur}
 
-inductive IsLiftableVector (rv: R) : (bs: List (LeftTypeBundled.{ur, ul} R)) → (Interleaving R bs) → List Bool → Prop where
-  | nil : IsLiftableVector rv [] (Interleaving.nil) []
-  | cons_true (b: LeftTypeBundled R) (bs: List (LeftTypeBundled R)) (il: Interleaving R bs)
-              (b2: b.liftableEmbedding.IsLiftable rv) (bs2: List Bool)
-        : IsLiftableVector rv bs il bs2 → IsLiftableVector rv (b::bs) (il.cons b) (.true::bs2)
-  | cons_false (b: LeftTypeBundled R) (bs: List (LeftTypeBundled R)) (il: Interleaving R bs)
-               (b2: ¬b.liftableEmbedding.IsLiftable rv) (bs2: List Bool)
-        : IsLiftableVector rv bs il bs2 → IsLiftableVector rv (b::bs) (il.cons b) (.false::bs2)
-
 
 end Interleaving
-
+-/
 
 
 
