Nemonuri/Functions/LiftableEmbedding/PSigma.lean
@@ -1,0 +1,34 @@
+module
+
+public import Nemonuri.Functions.LiftableEmbedding.Pi
+
+@[expose] public section
+
+set_option autoImplicit false
+
+namespace Nemonuri.Functions.LiftableEmbedding
+
+variable {L R: Sort*}
+
+--#check PSigma.mk
+
+def embedPSigma (lem: LiftableEmbedding L R) (mr: (rv: R) → Sort*) : (lv : L) ×' mr (lem lv) → ((rv: R) ×' mr rv)
+  | ⟨lv1, lv2⟩ => ⟨lem lv1, lv2⟩
+
+theorem embedPSigma_injective {lem: LiftableEmbedding L R} {mr: (rv: R) → Sort*} : Function.Injective (lem.embedPSigma mr) := by
+  intro psl1 psl2 lm1
+  simp [embedPSigma] at lm1
+  refine PSigma.ext ?_ ?_
+  · exact lm1.1
+  · exact lm1.2
+
+
+
+/-
+def comapPSigma (lem: LiftableEmbedding L R) (mr: (rv: R) → Sort*) : ((rv: R) ×' mr rv) → (lv : L) ×' mr (lem lv)
+  | ⟨fstR, sndR⟩ =>
+-/
+
+end Nemonuri.Functions.LiftableEmbedding
+
+end
